\title{Homework 2 COM S 311 }
\author{Alec Meyer}

\date{\today}

\documentclass[11pt]{article}
\newcommand\tab[1][1cm]{\hspace*{#1}}
\usepackage{amssymb}
\usepackage{listings}

\begin{document}
\maketitle



\section*{Question 1}
a.\\*
\tab $2^{2n} \in O(2^n)$\\*\\*
\tab Claim: $2^{2n} \notin O(2^n)$\\*\\*
\tab $f(n) \leq c \times g(n)$\\*\\*
\tab f(n) = $2^{2n}$, g(n) = $2^n$\\*\\*
\tab plug in f(n) and g(n)\\*
\tab $2^{2n} \leq c \times 2^n$\\*
\tab $\frac{2^{2n}}{2^n} \leq c$\\*
\tab $2^n \leq c$\\*\\*
\tab Here we have a constant 'c' being greater 
than or equal to a function of n. This is not 
possible as $2^n$ will surpass the value of c.
Therefore, since there is no constant value c
to satisfy this claim we know that this statement
is false.\\*
\tab $\therefore 2^{2n} \notin O(2^n)$\*
b.\\*\\*\\*


\section*{Question 2}
a.\\*
\tab Inner:\\*
\tab $$\sum_{k=1}^{j} c_1 = c_1j$$\\*
\tab Middle:\\*
\tab $$\sum_{j=i}^{n} (c_2 + c_1j)$$\\*
\tab $$\sum_{j=i}^{n} {c_2 + \sum_{j=i}^{n} c_1j}$$\\*
\tab $$\sum_{j=i}^{n} {c_1j} = c_1(\frac{n(n+1)}{2} - \frac{i(i-1)}{2}$$\\*
\tab $$\sum_{j=i}^{n} {c_2} = c_2(n - i + 1)$$\\*
\tab Outer:\\*
\tab $$\sum_{i=1}^{n-1}[c_2(n - i + 1) + c_1(\frac{n(n+1)}{2} - \frac{i(i-1)}{2})]$$\\*
\tab $$\sum_{i=1}^{n-1}[c_2n - c_2i + c_2 + \frac{c_1n^2}{2} + \frac{c_1n}{2} - \frac{c_1i^2}{2} - \frac{c_1i}{2}]$$\\*
\tab$$ = c_2n^2 - \frac{c_2n(n+1)}{2} - 1 + c_2 + \frac{c_1n^3}{2} + \frac{c_1n^2}{2} - \frac{n^2(n+1)}{2} - 1 - \frac{n(n+1)}{2} - 1$$\\*
\tab $$\in O(n^3)$$\\*


\section*{Question 3}
a.\\*
\begin{lstlisting}
for(int i = 0; i < A.size; i++)
	if(binarySearch(T-A[i]))
		TRUE
FALSE
\end{lstlisting}

\tab FOR loop time:\\*
\tab $$\sum_{i=0}^{n}Binary Search$$\\*
\tab We know that Binary Search is O(logn)\\*
\tab Binary Search runs n times, therefore the
runtime of this algorithm is O(nlogn)\\*
\end{document}